yalla/bug_report_2_bis.v
@@ -50,5 +50,5 @@ Restart.
   Fail Time done. (* Timeout! *) (* Takes more than 200 secs *)
   by unfold walk.
 Time Qed. (* Finished transaction in 0.008 secs (0.008u,0.s) (successful)*)
-
+(* TODO time if add more +1? *)
 End LongComputation.
